Makefile
@@ -46,9 +46,6 @@ endif
 
 UINT := $(shell coqc -config | grep COQLIB | cut -f2 -d'=')/kernel
 
-
-
-
 src/prover.cmx : src/prover.ml
 	ocamlc -annot -I $(UINT) -rectypes -c src/prover.mli
 	ocamlc -annot -I $(UINT) -I src -rectypes -c src/prover.ml
@@ -71,7 +68,7 @@ clean : cleanaux
 
 
 
-TESTSUITE = arith.v  refl_bool.v # no_test.v
+TESTSUITE = arith.v  refl_bool.v no_test.v
 ISSUES    = issue_0.v issue_2.v issue_3.v issue_5.v issue_6.v issue_8.v issue_9.v issue_10.v \
 	issue_11.v issue_12.v issue_13.v issue_14.v issue_15.v issue_16.v issue_19.v issue_20.v issue_21.v \
 	issue_22.v issue_23.v issue_cc.v
